begin porting event example

new_example/event.go
@@ -1,0 +1,34 @@
+package main
+
+import (
+	"github.com/tchajed/marshal"
+)
+
+type Event struct {
+	id        uint32
+	name      string
+	startTime TimeStamp
+	endTime   TimeStamp
+}
+
+func MarshalEvent(enc []byte, e Event) []byte {
+	enc = marshal.WriteInt32(enc, e.id)
+	enc = marshal.WriteLenPrefixedBytes(enc, []byte(e.name))
+	enc = MarshalTimeStamp(enc, e.startTime)
+	enc = MarshalTimeStamp(enc, e.endTime)
+	return enc
+}
+
+func UnmarshalEvent(s []byte) (Event, []byte) {
+	id, s := marshal.ReadInt32(s)
+	nameBytes, s := marshal.ReadLenPrefixedBytes(s)
+
+	startTime, s := UnmarshalTimeStamp(s)
+	endTime, s := UnmarshalTimeStamp(s)
+	return Event{
+		id:        id,
+		name:      string(nameBytes),
+		startTime: startTime,
+		endTime:   endTime,
+	}, s
+}
