new_example/event_proof.v
@@ -1,0 +1,48 @@
+From New.proof Require Import proof_prelude.
+From Grackle.new_ex Require Import goose.github_com.mjschwenne.grackle.new_example.
+From Grackle.new_ex Require Import pg.github_com.mjschwenne.grackle.new_example.
+From New.proof Require Import github_com.tchajed.marshal.
+From Grackle.new_ex Require Import timestamp_proof.
+
+Module Event_Proof.
+  Section Event_Proof.
+
+    Context `{hG: heapGS Σ, !ffi_semantics _ _}.
+    Context `{!goGlobalsGS Σ}.
+
+    #[global]
+      Program Instance : IsPkgInit main :=
+        ltac2:(build_pkg_init ()).
+
+    Definition has_encoding (encoded:list u8) (args:main.Event.t) : Prop :=
+      ∃ start_enc end_enc,
+        encoded = (u32_le args.(main.Event.id')) ++
+                    (u64_le $ length $ args.(main.Event.name')) ++
+                    args.(main.Event.name') ++
+                    start_enc ++ end_enc
+        /\ TimeStamp_Proof.has_encoding start_enc args.(main.Event.startTime')
+        /\ TimeStamp_Proof.has_encoding end_enc args.(main.Event.endTime').
+
+    Lemma wp_Encode (args__c:main.Event.t) (pre_sl:slice.t) (prefix:list u8) (dq:dfrac):
+      {{{
+            is_pkg_init main ∗
+            own_slice pre_sl (DfracOwn 1) prefix ∗
+            own_slice_cap w8 pre_sl
+      }}}
+        main @ "MarshalEvent" #pre_sl #args__c
+      {{{
+            enc enc_sl, RET #enc_sl;
+            ⌜ has_encoding enc args__c ⌝ ∗
+            own_slice enc_sl (DfracOwn 1) (prefix ++ enc) ∗
+            own_slice_cap w8 enc_sl
+      }}}.
+
+    Proof.
+      wp_start as "[Hsl Hcap]". wp_auto.
+
+      wp_apply (wp_WriteInt32 with "[$Hsl $Hcap]").
+      iIntros (?) "[Hsl Hcap]". wp_auto.
+
+    Admitted.
+  End Event_Proof.
+End Event_Proof.
